Protocol/tuple-marshalling/Program.fs
@@ -1,0 +1,10 @@
+﻿// Learn more about F# at http://fsharp.net
+// See the 'F# Tutorial' project for more help.
+open System
+[<EntryPoint>]
+let main argv = 
+    X.test "me"
+    printfn "Done" 
+    (* ignore <| Console.Read() *) //removing this just so that test runs to completion without kb input
+    0 //integer exit code
+
