Protocol/Network.fst
@@ -4,10 +4,10 @@ open Lib
 open Protocol
 
 (*Dummy implementation of actual networking*)
-(*open DummyNetwork*)
+open DummyNetwork
 
 (*This is the reference to the implementation in F#
-	This ic commented out for now to avoid struggeling with interop*)
+	This ic commented out for now to avoid struggeling with interop
 extern reference Network {language="F#";
 						dll="RuntimeExtention";
 						namespace="";
@@ -16,7 +16,7 @@ extern Network val SendResponse: prin -> list string -> string -> bool
 extern Network val SendRequest: uri -> list string -> string -> bool
 extern Network val RecieveResponse: prin -> (int *string * list string)
 extern Network val RecieveRequest: prin -> (string * string * string * list string)
-
+*)
 
 type HttpMessage =
 	| Get: uri -> list (string * string) -> list (string * string) -> HttpMessage
